src/Bitstream.v
@@ -19,3 +19,22 @@ Inductive n_bits : nat -> list val -> Prop :=
     forall n l b,
       n_bits n l ->
       n_bits (S n) (bit b :: l).
+
+
+Require Import Eager.
+Require Import List.
+
+
+Lemma n_bits_eval :
+  forall n x ge,
+    n_bits n x ->
+    exists v,
+      eager_eval_expr ge sempty (EList (map EValue x)) v.
+Proof.
+  induction 1; intros.
+  eexists. econstructor; eauto. simpl. econstructor.
+  destruct IHn_bits.
+  inversion H0.
+  eexists. simpl. econstructor. simpl. econstructor. econstructor. econstructor.
+  eauto. reflexivity.
+Qed.
