src/BuiltinSyntax.v
@@ -1,0 +1,98 @@
+Require Import List.
+Require Import String.
+
+Require Import Coqlib.
+
+Require Import AST.
+Require Import Builtins.
+Require Import Values.
+Require Import Bitvectors.
+
+Open Scope string.
+
+
+Fixpoint make_arg_list (n : nat) : list Expr :=
+  match n with
+  | O => nil
+  | S n' => (EVar (Z.of_nat n, "")) :: make_arg_list n'
+  end.
+
+Fixpoint iter {A : Type} (n : nat) (f : nat -> A -> A) (b : A) : A :=
+  match n with
+  | O => b
+  | S n' => f n (iter n' f b)
+  end.
+
+Definition mb (num_type_args : nat) (num_args : nat) (b : builtin) : Expr :=
+  let l := make_arg_list (num_args + num_type_args) in 
+  let raw_e := iter num_args (fun n => fun x => EAbs (Z.of_nat n, "") x) (EBuiltin b l) in
+  let t_e := iter num_type_args (fun n => fun x => ETAbs ((Z.of_nat (n + num_args )), "") x) raw_e in
+  t_e.
+
+
+(* table of builtins, along with their arity *)
+(* mb 9 9 _ indicates hasn't been implemented, will break when tested *)
+Definition table : list (string * Expr) :=
+  ("demote", mb 2 0 Demote) :: 
+  ("+", mb 1 2 Plus) :: (* TESTED *)
+  ("-", mb 1 2 Minus) :: 
+  ("*", mb 1 2 Times) :: 
+  ("/", mb 1 2 Div) :: 
+  ("%", mb 1 2 Mod) :: 
+  ("^^", mb 1 2 Exp) :: (* Underlying op not implemented *)
+  ("lg2", mb 1 2 lg2) :: (* Underlying op not implemented *)
+  ("True", mb 0 0 true_builtin) :: (* TESTED *)
+  ("False", mb 0 0 false_builtin) :: (* TESTED *)
+  ("negate", mb 1 1 Neg) :: 
+  ("complement", mb 1 1 Compl) :: 
+  ("<", mb 1 2 Lt) :: 
+  (">", mb 1 2 Gt) :: 
+  ("<=", mb 1 2 Le) ::
+  (">=", mb 1 2 Ge) ::
+  ("==", mb 1 2 Eq) ::
+  ("!=", mb 1 2 Neq) ::
+  ("&&", mb 1 2 And) ::
+  ("||", mb 1 2 Or) :: 
+  ("^", mb 1 2 Xor) :: 
+  ("zero", mb 1 0 Zero) :: 
+  ("<<", mb 1 2 Shiftl) :: 
+  (">>", mb 1 2 Shiftr) :: 
+  ("<<<", mb 1 2 Rotl) :: 
+  (">>>", mb 1 2 Rotr) :: 
+  ("#", mb 3 2 Append) :: 
+  ("splitAt", mb 3 1 splitAt) :: 
+  ("join", mb 9 9 join) :: (* Not yet implemented *)
+  ("split", mb 3 1 split) :: 
+  ("reverse", mb 9 9 reverse) :: (* Not yet implemented *)
+  ("transpose", mb 9 9 transpose) :: (* Not yet implemented *)
+  ("@", mb 3 2 At) :: 
+  ("@@", mb 9 9 AtAt) :: (* Not yet implemented *)
+  ("!", mb 9 9 Bang) :: (* Not yet implemented *)
+  ("!!", mb 9 9 BangBang) :: (* Not yet implemented *)
+  ("update", mb 9 9 update) ::(* Not yet implemented *)
+  ("updateEnd", mb 9 9 updateEnd) :: (* Not yet implemented *)
+  ("fromThen", mb 9 9 fromThen) :: (* Not yet implemented *)
+  ("fromTo", mb 9 9 fromTo) :: (* Not yet implemented *)
+  ("fromThenTo", mb 9 9 fromThenTo) :: (* Not yet implemented *)
+  ("infFrom", mb 9 9 infFrom) :: (* Not yet implemented *)
+  ("infFromThen", mb 9 9 infFromThen) :: (* Not yet implemented *)
+(*  ("error", mb 9 9 error) :: (* Not yet implemented *)*)
+  ("pmult", mb 9 9 pmult) :: (* Not yet implemented *)
+  ("pdiv", mb 9 9 pdiv) :: (* Not yet implemented *)
+  ("pmod", mb 9 9 pmod) :: (* Not yet implemented *)
+(*  ("random", mb 9 9 random) :: (* Not going to be implemented *)*)
+(*  ("trace", mb 9 9 trace) :: (* Not going to be implemented *)*)
+  nil.
+
+Fixpoint lookup {A : Type} (s : string) (t : list (string * A)) : option A :=
+  match t with
+  | nil => None
+  | (n,a) :: r => if string_dec n s then Some a else lookup s r
+  end.
+
+Definition find_builtin (s : string) : option Expr :=
+  lookup s table.
+
+Definition lookup_prim (id : ident) : option Expr :=
+  let (_,n) := id in
+  find_builtin n.
