verif/Basic1.v
@@ -11,6 +11,7 @@ Require Import Semantics.
 Require Import Utils.
 Require Import Builtins.
 Require Import BuiltinSem.
+Require Import BuiltinSyntax.
 Require Import Values.        
 
 Require Import EvalTac.
@@ -22,7 +23,7 @@ Open Scope string.
 
 Definition z : ident := (244,"z").
 
-
+(*
 Lemma eval_z :
   exists v,
     eval_expr ge empty (EVar z) v /\ force_list ge empty v ([bit true, bit true]).
@@ -50,3 +51,4 @@ Proof.
 
   Unshelve. simpl; auto.
 Qed.
+*)
