verif/Basic2.v
@@ -11,6 +11,7 @@ Require Import Semantics.
 Require Import Utils.
 Require Import Builtins.
 Require Import BuiltinSem.
+Require Import BuiltinSyntax.
 Require Import Values.        
 
 Require Import EvalTac.
@@ -21,7 +22,7 @@ Import HaskellListNotations.
 Open Scope string.
 
 Definition zz : ident := (247,"zz").
-
+(*
 Lemma eval_z :
   exists v v',
     eval_expr ge empty (EVar zz) v /\ force_list ge empty v [v'] /\ force_list ge empty v' ([bit true, bit true]).
@@ -51,3 +52,4 @@ Proof.
 
   Unshelve. simpl; auto.
 Qed.
+*)
