verif/HMAC_verif.v
@@ -1,0 +1,105 @@
+Require Import List.
+Import ListNotations.
+Require Import String.
+
+(* Borrow from CompCert *)
+Require Import Coqlib.
+Require Import Bitvectors.
+
+Require Import AST.
+(*Require Import Semantics.*)
+Require Import Utils.
+Require Import Builtins.
+Require Import BuiltinSem.
+Require Import BuiltinSyntax.
+Require Import Values.        
+Require Import Eager.
+Require Import Bitstream.
+
+Require Import EvalTac.
+
+Import HaskellListNotations.
+Open Scope string.
+
+Require Import HMAC.
+
+Require Import HMAC_spec.
+
+(* Require Import Bvector.*)
+
+
+(* Eager tactics *)
+(* TODO: standardize *)
+Ltac ec := econstructor; try unfold mb; try reflexivity.
+Ltac fg := eapply eager_eval_global_var; [ reflexivity | eassumption | idtac].
+Ltac g := eapply eager_eval_global_var; try eassumption; try reflexivity.
+
+Ltac e :=
+  match goal with
+  | [ |- eager_eval_expr _ ?E (EVar ?id) _ ] =>
+    try fg; try reflexivity;
+    try solve [eapply eager_eval_local_var; reflexivity]
+  | [ |- _ ] => ec
+  end.
+
+Definition typenum (n : Z) : Expr := ETyp (TCon (TC (TCNum n)) []).
+Definition pwBytes := typenum 64.
+Definition blockLength := typenum 64.
+Definition digest := typenum 0.
+
+Fixpoint apply (e : Expr) (l : list Expr) : Expr :=
+  match l with
+  | nil => e
+  | f :: r => apply (EApp e f) r
+  end.
+
+Fixpoint tapply (e : Expr) (l : list Expr) : Expr :=
+  match l with
+  | nil => e
+  | f :: r => tapply (ETApp e f) r
+  end.
+
+
+Lemma kinit_eval :
+  forall k,
+    n_bits 64 k ->
+    forall h,
+    exists v,
+      eager_eval_expr ge sempty (apply (tapply (EVar kinit) (pwBytes :: blockLength :: digest ::  nil)) (h :: (EList (map EValue k)) :: nil)) v.
+Proof.
+  init_globals ge.
+  intros.
+  remember H as Hnb; clear HeqHnb.
+  eapply n_bits_eval in H; eauto.
+  destruct H. instantiate (1 := ge) in H.
+  
+  eexists. unfold apply.
+  e. e.
+  e. e. e. g. e. repeat e.
+  e. repeat e.
+  e. repeat e.
+  e.
+  admit. (* hash evaluates to some closure *)
+  e. 
+  eassumption.
+  e. e. e. e. g. e. repeat e.
+  e. e. e. e. repeat e. repeat e.
+  simpl. repeat e. repeat e. repeat e.
+  
+  e. e. e. e. e. repeat e.
+  e. repeat e. e. repeat e. simpl. reflexivity.
+  e. repeat e.
+  simpl. reflexivity.
+  simpl. e.
+  e. e. e. g. e. repeat e.
+  e. repeat e.
+  e. repeat e. e. e. e. repeat e.
+  e. e. e. g. e. repeat e. repeat e.
+  e. repeat e.
+
+
+  (* TODO: Prove that append works for x *)
+  (* TODO: add eager evaluation of where *)
+  
+  
+Admitted.
